Fixed bug.

Isabelle2/MultiPaxos4.thy
@@ -553,11 +553,11 @@ definition mp_asig where
 fun init_nodes_state where
   "init_nodes_state (0::nat) n = undefined"
 | "init_nodes_state (Suc i) n = 
-    (if Suc i > n then undefined else (init_nodes_state i n)(Suc i $:= init_acc_state n (Suc i)))"
+    (if Suc i > n then undefined else (init_nodes_state i n)(Suc i $:= def_IntEvtHandler_InitializeReplicaState n (Suc i)))"
 
 lemma init_acc: 
 assumes "a \<le> n" and "a > 0"
-shows "(init_nodes_state a n) $ a = init_acc_state n a" using assms
+shows "(init_nodes_state a n) $ a = def_IntEvtHandler_InitializeReplicaState n a" using assms
 by (induct a n arbitrary:n rule:init_nodes_state.induct, auto)
 
 
